Improve proof performance by making communication layer functions opaque and relying on lemmas (#102)
* Made most communication layer core functions opaque, added SMTPats

* Made reqres functions opaque

* Strength request send/receive postconditions

---------

Co-authored-by: Klaas Pruiksma <klaas.pruiksma@sec.uni-stuttgart.de>

src/lib/communication/DY.Lib.Communication.RequestResponse.Lemmas.fst
@@ -36,10 +36,10 @@ let comm_meta_data_knowable #cinvs tr prin req_meta_data =
   is_knowable_by (principal_label prin) tr req_meta_data.key /\
   is_knowable_by (principal_label prin) tr req_meta_data.request
 
-val apply_com_layer_lemmas: 
-  #a:Type -> {| parseable_serializeable bytes a |} -> 
+val apply_reqres_comm_layer_lemmas:
+  #a:Type -> {| parseable_serializeable bytes a |} ->
   comm_reqres_higher_layer_event_preds a -> prop
-let apply_com_layer_lemmas _ = True
+let apply_reqres_comm_layer_lemmas _ = True
 
 
 val send_request_proof:
@@ -60,13 +60,19 @@ val send_request_proof:
     is_well_formed a (is_knowable_by (comm_label client server) tr) request
   )
   (ensures (
-    let (_, tr_out) = send_request comm_keys_ids client server request tr in
-    trace_invariant tr_out
+    match send_request comm_keys_ids client server request tr with
+    | (None, tr_out) -> trace_invariant tr_out
+    | (Some (_, cmeta_data), tr_out) -> (
+      trace_invariant tr_out /\
+      comm_meta_data_knowable tr_out client cmeta_data
+    )
   ))
   [SMTPat (trace_invariant tr);
-  SMTPat (apply_com_layer_lemmas higher_layer_preds);
+  SMTPat (apply_reqres_comm_layer_lemmas higher_layer_preds);
   SMTPat (send_request comm_keys_ids client server request tr)]
 let send_request_proof #invs #a tr comm_keys_ids higher_layer_preds client server request =
+  reveal_opaque (`%send_request) (send_request #a);
+  assert(apply_core_comm_layer_lemmas request_response_event_preconditions);
   let request_bytes = serialize #bytes a request in
   match send_request comm_keys_ids client server request tr with
   | (None, tr_out) -> (
@@ -74,11 +80,10 @@ let send_request_proof #invs #a tr comm_keys_ids higher_layer_preds client serve
     let (sid, tr') = new_session_id client tr' in
     let ((), tr') = set_state client sid (ClientSendRequest {server; request=request_bytes; key} <: communication_states) tr' in
     higher_layer_preds.send_request_later tr tr' client server request (get_label tr' key);
-    let ((), tr') = trigger_event client (CommClientSendRequest client server request_bytes key) tr' in
     ()
   )
   | (Some _, tr_out) -> (
-    let (key, tr') = mk_rand (AeadKey comm_layer_aead_tag empty) (comm_label client server) 32 tr in   
+    let (key, tr') = mk_rand (AeadKey comm_layer_aead_tag empty) (comm_label client server) 32 tr in
     let (sid, tr') = new_session_id client tr' in
     let ((), tr') = set_state client sid (ClientSendRequest {server; request=request_bytes; key} <: communication_states) tr' in
     higher_layer_preds.send_request_later tr tr' client server request (get_label tr' key);
@@ -86,7 +91,6 @@ let send_request_proof #invs #a tr comm_keys_ids higher_layer_preds client serve
     assert(trace_invariant tr');
     let req_payload:com_message_t = RequestMessage {request=(serialize a request); key} in
     let req_payload_bytes = serialize #bytes com_message_t req_payload in
-    send_confidential_proof tr' request_response_event_preconditions comm_keys_ids client server req_payload;   
     let (Some msg_id, tr') = send_confidential comm_keys_ids client server req_payload tr' in
 
     assert(tr_out == tr');
@@ -120,14 +124,16 @@ val receive_request_proof:
       trace_invariant tr_out /\
       event_triggered tr_out server (CommServerReceiveRequest server payload_bytes req_meta_data.key) /\
       is_well_formed a (is_knowable_by (principal_label server) tr_out) payload /\
-      is_well_formed a (is_knowable_by (get_response_label tr_out req_meta_data) tr_out) payload
+      is_well_formed a (is_knowable_by (get_response_label tr_out req_meta_data) tr_out) payload /\
+      payload_bytes == req_meta_data.request
     )
   ))
   [SMTPat (trace_invariant tr);
-  SMTPat (apply_com_layer_lemmas higher_layer_preds);
+  SMTPat (apply_reqres_comm_layer_lemmas higher_layer_preds);
   SMTPat (receive_request #a comm_keys_ids server msg_id tr)]
 let receive_request_proof #invs #a tr comm_keys_ids higher_layer_preds server msg_id =
-  receive_confidential_proof #invs tr request_response_event_preconditions comm_keys_ids server msg_id;
+  reveal_opaque (`%receive_request) (receive_request #a);
+  assert(apply_core_comm_layer_lemmas request_response_event_preconditions);
   match receive_request #a comm_keys_ids server msg_id tr with
   | (None, tr_out) -> ()
   | (Some (payload, req_meta_data), tr_out) -> (
@@ -188,7 +194,8 @@ val mk_comm_layer_response_nonce_proof:
       is_knowable_by (get_response_label tr_out req_meta_data) tr_out nonce
     )
   ))
-let mk_comm_layer_response_nonce_proof #invs tr req_meta_data usg = ()
+let mk_comm_layer_response_nonce_proof #invs tr req_meta_data usg =
+  reveal_opaque (`%mk_comm_layer_response_nonce) (mk_comm_layer_response_nonce)
 
 
 val compute_response_message_proof:
@@ -201,7 +208,7 @@ val compute_response_message_proof:
   (requires
     has_communication_layer_reqres_crypto_predicates /\
     is_knowable_by (principal_label server) tr key /\
-    is_well_formed a (is_knowable_by (get_label tr key) tr) response /\    
+    is_well_formed a (is_knowable_by (get_label tr key) tr) response /\
     is_publishable tr nonce /\
     key `has_usage tr` (AeadKey comm_layer_aead_tag empty) /\
     event_triggered tr server (CommServerSendResponse server request (serialize a response))
@@ -210,12 +217,13 @@ val compute_response_message_proof:
     is_publishable tr (compute_response_message #a server key nonce response)
   )
 let compute_response_message_proof #cinvs #a tr server key nonce request response =
+  reveal_opaque (`%compute_response_message) (compute_response_message #a);
   let res_bytes = serialize a response in
   serialize_wf_lemma a (is_knowable_by (get_label tr key) tr) response;
   let ad:authenticated_data = {server} in
   let ad_bytes = serialize authenticated_data ad in
   serialize_wf_lemma authenticated_data (is_publishable tr) ad;
-  let ciphertext = aead_enc key nonce res_bytes ad_bytes in  
+  let ciphertext = aead_enc key nonce res_bytes ad_bytes in
   // Needed for the case that the key is publishable
   FStar.Classical.move_requires (aead_enc_preserves_publishability tr key nonce res_bytes) ad_bytes;
   serialize_wf_lemma com_message_t (is_publishable tr) (ResponseMessage {nonce; ciphertext});
@@ -243,15 +251,16 @@ val send_response_proof:
     trace_invariant tr_out
   ))
   [SMTPat (trace_invariant tr);
-  SMTPat (apply_com_layer_lemmas higher_layer_preds);
+  SMTPat (apply_reqres_comm_layer_lemmas higher_layer_preds);
   SMTPat (send_response server req_meta_data response tr)]
 let send_response_proof #invs #a tr higher_layer_preds server req_meta_data response =
+  reveal_opaque (`%send_response) (send_response #a);
   match send_response server req_meta_data response tr with
   | (None, tr_out) -> ()
   | (Some msg_id, tr_out) -> (
     let (Some state, tr') = get_state server req_meta_data.sid tr in
-    let ServerReceiveRequest srr = state in    
-    let ((), tr') = trigger_event server (CommServerSendResponse server req_meta_data.request (serialize a response)) tr' in    
+    let ServerReceiveRequest srr = state in
+    let ((), tr') = trigger_event server (CommServerSendResponse server req_meta_data.request (serialize a response)) tr' in
     let (nonce, tr') = mk_rand NoUsage public 32 tr' in
     compute_response_message_proof tr' server req_meta_data.key nonce req_meta_data.request response;
     let resp_msg_bytes = compute_response_message server req_meta_data.key nonce response in
@@ -287,6 +296,7 @@ val decode_response_proof:
     )
   ))
 let decode_response_proof #cinvs #a #ps tr client server key msg_bytes =
+  reveal_opaque (`%decode_response_message) (decode_response_message #a);
   match decode_response_message #a server key msg_bytes with
   | None -> ()
   | Some payload -> (
@@ -325,9 +335,10 @@ val receive_response_proof:
     )
   ))
   [SMTPat (trace_invariant tr);
-  SMTPat (apply_com_layer_lemmas higher_layer_preds);
+  SMTPat (apply_reqres_comm_layer_lemmas higher_layer_preds);
   SMTPat (receive_response #a client req_meta_data msg_id tr)]
 let receive_response_proof #invs #a tr higher_layer_preds client req_meta_data msg_id =
+  reveal_opaque (`%receive_response) (receive_response #a);
   match receive_response #a client req_meta_data msg_id tr with
   | (None, tr_out) -> ()
   | (Some (response, _), tr_out) -> (
